theory/JITPer_add_imm.thy
@@ -1,0 +1,197 @@
+theory JITPer_add_imm
+imports
+  Main
+  rBPFCommType rBPFSyntax rBPFSem
+  x64Syntax x64Semantics x64Assembler
+  JITPer_aux
+
+begin
+
+lemma aluq_imm_subgoal_rr_aux1:
+     "bins = BPF_ALU64 BPF_ADD dst (SOReg src) \<Longrightarrow>
+     xins = Paddq_rr (bpf_to_x64_reg dst) (bpf_to_x64_reg src) \<Longrightarrow>
+     prog!(unat pc) = bins \<Longrightarrow>
+     sbpf_step prog (SBPF_OK pc rs m ss) = (SBPF_OK pc' rs' m' ss')  \<Longrightarrow>
+     Next spc' reg' xm' xss' = exec_instr xins sz spc reg xm xss \<Longrightarrow>
+     reg (IR (bpf_to_x64_reg dst)) = rs dst \<Longrightarrow>
+     reg (IR (bpf_to_x64_reg src)) = rs src \<Longrightarrow>
+     reg' (IR (bpf_to_x64_reg dst)) = (rs' dst)"
+  apply (unfold exec_instr_def step)
+  apply simp
+  apply(cases "prog ! unat pc",simp_all)
+  subgoal for x91 apply(simp split:if_split_asm) 
+    apply(unfold eval_alu_def eval_reg_def,simp_all)
+    by auto
+  done
+
+
+lemma aluq_imm_subgoal_rr_aux2_1:"xins = Paddq_rr dst src \<Longrightarrow> 
+  Next pc' reg' m' xss' = exec_instr xins sz pc reg m xss \<Longrightarrow>
+  \<forall> r \<noteq> dst. reg' (IR r) = reg (IR r)"
+  by (simp add: exec_instr_def)
+
+
+lemma aluq_imm_subgoal_rr_aux2:"xins = Paddq_rr (bpf_to_x64_reg dst) (bpf_to_x64_reg src) \<Longrightarrow> 
+  Next pc' reg' m' xss' = exec_instr xins sz pc reg m xss \<Longrightarrow>
+  \<forall> r \<noteq> dst. reg' (IR (bpf_to_x64_reg r)) = reg (IR (bpf_to_x64_reg r))"
+  using aluq_imm_subgoal_rr_aux2_1 by simp
+
+
+
+lemma aluq_imm_subgoal_rr_aux3:"bins = BPF_ALU64 BPF_ADD dst (SOReg src) \<Longrightarrow> 
+  sbpf_step prog (SBPF_OK pc rs m ss) = (SBPF_OK pc' rs' m' ss') \<Longrightarrow> 
+  prog!(unat pc) = bins \<Longrightarrow>
+  \<forall> r \<noteq> dst. rs' r = rs r"
+  apply(cases bins,simp_all)
+  apply(cases "prog ! unat pc", simp_all)
+  subgoal for x91 apply(simp split:if_split_asm) 
+    apply(unfold eval_alu_def eval_reg_def,simp_all)
+    by auto
+  done
+
+lemma stack_is_not_changed_by_add:"Next spc' reg' m' xss' = exec_instr xins sz spc reg m xss \<Longrightarrow> xins = Paddq_rr (bpf_to_x64_reg dst) (bpf_to_x64_reg src) 
+   \<Longrightarrow> match_stack reg \<Longrightarrow> match_stack reg' "
+proof-
+  assume a0:"Next spc' reg' m' xss' = exec_instr xins sz spc reg m xss" and
+  a1:"xins = Paddq_rr (bpf_to_x64_reg dst) (bpf_to_x64_reg src) " and
+  a2:"match_stack reg"
+  have b0:"bpf_to_x64_reg dst \<noteq> RSP" using bpf_to_x64_reg_def by (cases dst,simp_all)
+  have b1:"reg (IR SP) = reg' (IR SP)" using exec_instr_def a0 a1 b0
+    by (metis (no_types, opaque_lifting) aluq_imm_subgoal_rr_aux2_1)
+  have "match_stack reg' " using b1 a2 match_stack_def by auto
+  thus ?thesis by blast
+qed
+
+lemma mem_is_not_changed_by_add:"Next spc' reg' m' xss'= exec_instr xins sz spc reg m xss\<Longrightarrow> xins = Paddq_rr (bpf_to_x64_reg dst) (bpf_to_x64_reg src) 
+   \<Longrightarrow> m = m'"
+  using exec_instr_def by simp
+
+(*value "((scast (scast (-1::i32)::u32))::u64)"
+value "((scast ((-1)::i32))::u64)"*)
+
+
+lemma scast_aux1:"((scast (scast (imm::i32)::u32))::u64) = ((scast imm)::u64)"
+  sorry
+
+(*(\<And>(r::ireg) dst::bpf_ireg. r = bpf_to_x64_reg dst \<Longrightarrow> bpf_to_x64_reg dst \<noteq> REG_OTHER_SCRATCH) \<Longrightarrow> *)
+lemma addq_imm_one_step_match_reg:
+  " (SBPF_OK pc' rs' m' ss') = sbpf_step prog (SBPF_OK pc rs m ss) \<Longrightarrow>
+    xst = (Next xpc xrs xm xss) \<Longrightarrow>
+    match_state (SBPF_OK pc rs m ss) (pc,xst) \<Longrightarrow>
+    prog \<noteq> [] \<and> unat pc < length prog \<and> unat pc \<ge> 0 \<Longrightarrow>
+    prog!(unat pc) = BPF_ALU64 BPF_ADD dst (SOImm (imm::i32)) \<Longrightarrow>
+    bpf_to_x64_reg dst \<noteq> REG_OTHER_SCRATCH \<Longrightarrow> 
+    match_reg rs' ((\<lambda>a::preg. if a = IR REG_OTHER_SCRATCH then (scast ((scast (imm::i32))::u32))::u64 else xrs a)(IR (bpf_to_x64_reg dst) := xrs (IR (bpf_to_x64_reg dst)) + (scast ((scast (imm::i32))::u32))::u64))"
+  apply (simp add: match_state_def match_reg_def eval_alu_def eval_alu64_aux2_def eval_reg_def)
+  apply rule apply rule 
+  subgoal for r apply rule using scast_aux1 by presburger 
+  subgoal for r apply rule apply rule using reg_r10_consist by simp
+  done
+
+
+
+lemma addq_imm_one_step:
+ assumes a0:"s' = sbpf_step prog s" and
+  a1:"s = (SBPF_OK pc rs m ss)" and
+  a2:"s' = (SBPF_OK pc' rs' m' ss')" and
+  a3:"xst = (Next xpc xrs xm xss)" and
+  a4:"match_state s (pc,xst)" and
+  a5:"jitper prog = Some x64_prog" and                      
+  a6:"prog \<noteq> [] \<and> unat pc < length prog \<and> unat pc \<ge> 0" and
+  a8:"prog!(unat pc) = BPF_ALU64 BPF_ADD dst (SOImm (imm::i32))" 
+shows "\<exists> xst'. perir_sem 1 x64_prog (pc,xst) = (pc',xst') \<and> 
+  match_state s' (pc',xst')"
+  apply simp
+
+(* 1. as BPF_ADD generates a single list of jited x64 assembly, so we only need one step  *)
+  apply(subgoal_tac "\<exists>xst'::outcome. perir_step x64_prog (pc, xst) = (pc', xst') \<and> match_state s' (pc', xst')")
+  subgoal
+    by auto
+  subgoal
+    apply (unfold perir_step_def Let_def)
+(* 2. according to the code structure of JITPer, removing the first case statement *)
+    apply(subgoal_tac "x64_prog ! unat (fst (pc, xst)) = the (per_jit_add_imm64_1 dst (imm::i32))")
+     prefer 2
+    subgoal
+      using a5 a6 a8 aux5 per_jit_ins_def by fastforce
+    subgoal
+      apply (subgoal_tac "the (per_jit_add_imm64_1 dst (imm::i32)) = (2, 0, x64_encode (Pmovl_ri R10 (scast (imm::i32)))@x64_encode (Paddq_rr (bpf_to_x64_reg dst) R10))")
+       prefer 2
+      subgoal by (simp add: per_jit_add_imm64_1_def)
+      apply (subgoal_tac "(x64_encode (Pmovl_ri R10 (scast (imm::i32)::u32))@x64_encode (Paddq_rr (bpf_to_x64_reg dst) R10)) !1 \<noteq> 0x39 \<and> 
+        (x64_encode (Pmovl_ri R10 (scast (imm::i32)))@x64_encode (Paddq_rr (bpf_to_x64_reg dst) R10)) !0 \<noteq> 0xc3 \<and> 
+        (x64_encode (Pmovl_ri R10 (scast (imm::i32)))@x64_encode (Paddq_rr (bpf_to_x64_reg dst) R10)) !0 \<noteq> 0xe8")
+       prefer 2
+      subgoal apply(unfold x64_encode_def) 
+        apply(cases "Pmovl_ri R10 (scast (imm::i32)::u32)",simp_all) 
+        subgoal for x11 apply(unfold per_jit_add_imm64_1_def construct_rex_to_u8_def bitfield_insert_u8_def Let_def u8_of_bool_def,simp_all)
+          done
+        done
+      subgoal
+        unfolding a3
+        apply simp
+        apply (erule subst)
+        apply (erule subst)
+        apply (subgoal_tac "Suc 1 = (2::nat)") prefer 2 subgoal by simp
+        apply (erule subst [of _ 2])
+        apply (simp only: x64_sem.simps)
+(* 3. here we get a simplified version, next step is to remove another case statement *)
+        apply (subgoal_tac "x64_decode 0 (x64_encode (Pmovl_ri R10 (scast imm))@x64_encode (Paddq_rr (bpf_to_x64_reg dst) R10)) = Some (7, Pmovl_ri R10 (scast imm))")
+         prefer 2
+        subgoal
+          apply (rule_tac l_bin = "(x64_encode (Pmovl_ri R10 (scast imm)))" in x64_encode_decode_consistency)
+          subgoal using list_in_list_prop  
+            using list_in_list_concat by blast
+          subgoal by simp
+          subgoal using x64_encode_def construct_rex_to_u8_def bitfield_insert_u8_def Let_def u8_list_of_u32_def
+            by fastforce
+          done
+        subgoal
+          apply simp
+          apply (erule subst)
+          apply (simp add: exec_instr_def)
+          apply (subgoal_tac "Suc 0 = (1::nat)") prefer 2 subgoal by simp
+          apply (erule subst [of _ 1])
+          apply (simp only: x64_sem.simps)
+
+       apply (subgoal_tac "x64_decode (7::nat)
+            (x64_encode (Pmovl_ri R10 (scast imm))@x64_encode (Paddq_rr (bpf_to_x64_reg dst) R10))
+            = Some (3, Paddq_rr (bpf_to_x64_reg dst) R10)")
+           prefer 2
+           apply(subgoal_tac "length(x64_encode (Paddq_rr (bpf_to_x64_reg dst) R10)) = 3")
+            prefer 2 subgoal using x64_encode_def construct_rex_to_u8_def bitfield_insert_u8_def Let_def u8_list_of_u32_def by auto
+          subgoal 
+            apply (rule_tac l_bin = "x64_encode (Paddq_rr (bpf_to_x64_reg dst) R10)" in x64_encode_decode_consistency)
+          subgoal using list_in_list_prop_aux2
+            by (metis \<open>(x64_encode (Pmovl_ri REG_OTHER_SCRATCH (scast (imm::32 signed word))) @ x64_encode (Paddq_rr (bpf_to_x64_reg (dst::bpf_ireg)) REG_OTHER_SCRATCH)) ! Suc (0::nat) \<noteq> (57::8 word) \<and> (x64_encode (Pmovl_ri REG_OTHER_SCRATCH (scast imm)) @ x64_encode (Paddq_rr (bpf_to_x64_reg dst) REG_OTHER_SCRATCH)) ! (0::nat) \<noteq> (195::8 word) \<and> (x64_encode (Pmovl_ri REG_OTHER_SCRATCH (scast imm)) @ x64_encode (Paddq_rr (bpf_to_x64_reg dst) REG_OTHER_SCRATCH)) ! (0::nat) \<noteq> (232::8 word) \<Longrightarrow> x64_decode (0::nat) (x64_encode (Pmovl_ri REG_OTHER_SCRATCH (scast imm)) @ x64_encode (Paddq_rr (bpf_to_x64_reg dst) REG_OTHER_SCRATCH)) = Some (7::nat, Pmovl_ri REG_OTHER_SCRATCH (scast imm))\<close> append.right_neutral append_Nil list.size(3) option.sel prod.sel(1) x64_encode_decode_consistency)
+          subgoal by simp
+          subgoal apply (erule subst) 
+            using x64_encode_def construct_rex_to_u8_def bitfield_insert_u8_def Let_def
+            by fastforce
+          done
+        apply simp
+        apply (erule subst)
+        apply (simp add: exec_instr_def)
+        apply (subgoal_tac "bpf_to_x64_reg dst \<noteq> R10")
+        prefer 2 subgoal
+          using reg_r10_consist by simp
+        apply simp
+
+(* 4. now we get exec_instr (one step of x64 add assembly), we prove the \<and>, first left, then right *)
+          apply (rule conjI)
+          subgoal
+            using a0 a1 a2 a5 a6 a8 corr_pc_aux2 insert_iff prod_cases3 by metis
+          subgoal
+            unfolding a1 a2
+            apply (simp add: match_state_def)
+            apply (rule conjI)
+            subgoal using addq_imm_one_step_match_reg a0 a1 a2 a3 a4 a5 a6 a8 
+            by (metis a0 a1 a2 a3 a4 a8 list_in_list_prop match_state_eqiv per_jit_add_reg64_1_def x64_encode_decode_consistency)
+          done
+        done
+      done
+    done
+  done
+
+
+end
